% -*- mode: context; -*-
\chapter{Summation of Trigonometric Series}
\section{Problems}
\startitemize[n, 1*broad]
\item Multiplying both sides by $2\sin\frac{\beta}{2}$ and writing termwise, we get
  \startformula\startalign
    \NC 2\sin\alpha\sin\frac{\beta}{2} \NC = \cos\left(\alpha - \frac{\beta}{2}\right) - \cos\left(\alpha +
    \frac{\beta}{2}\right)\NR
    \NC 2\sin(\alpha + \beta)\sin\frac{\beta}{2} \NC = \cos\left(\alpha + \frac{\beta}{2}\right) -
    \cos\left(\alpha + \frac{3\beta}{2}\right)\NR
    \NC 2\sin(\alpha + 2\beta)\sin\frac{\beta}{2} \NC = \cos\left(\alpha + \frac{3\beta}{2}\right) -
    \cos\left(\alpha + \frac{5\beta}{2}\right)\NR
    \NC \NC \cdots\NR
    \NC 2\sin(\alpha + (n - 1)\beta)\sin\frac{\beta}{2} \NC = \cos\left(\alpha + (2n - 3)\frac{\beta}{2}\right)
    - \cos\left(\alpha + (2n - 1)\frac{\beta}{2}\right)\NR
  \stopalign\stopformula

  Adding we get $2\left[\sin\frac{\beta}{2}\sin\alpha + \sin(\alpha + \beta) + \sin(\alpha + 2\beta) + \cdots +
  \sin(\alpha + (n - 1)\beta)\right] = \cos\left(\alpha - \frac{\beta}{2}\right) - \cos\left[\alpha + (2n -
    1)\frac{\beta}{2}\right]$

  $\Rightarrow \sin\alpha + \sin(\alpha + \beta) + \sin(\alpha + 2\beta) + \cdots + \sin(\alpha + (n -
  1)\beta) = \frac{\sin\frac{n\beta}{2}}{\sin\frac{\beta}{2}}\sin\left[\alpha + (n -
    1)\frac{\beta}{2}\right]$
\item Let $S = cos\alpha + \cos(\alpha + \beta) + \cos(\alpha + 2\beta) + \cdots + \cos(\alpha + (n -
  1)\beta)$

  Multiplyinf both sides by $2\sin\frac{\beta}{2}$ like previous problems and writing termwise

  \startformula\startalign
    \NC 2\cos\alpha\sin\frac{\beta}{2} \NC = \sin\left(\alpha + \frac{\beta}{2}\right) - \sin\left(\alpha -
    \frac{\beta}{2}\right)\NR
    \NC 2\cos(\alpha + \beta)\sin\frac{\beta}{2} \NC = \sin\left(\alpha + \frac{3\beta}{2}\right) -
    \sin\left(\alpha + \frac{\beta}{2}\right)\NR
    \NC 2\cos(\alpha + 2\beta)\sin\frac{\beta}{2} \NC = \sin\left(\alpha + \frac{5\beta}{2}\right) -
    \sin\left(\alpha + \frac{3\beta}{2}\right)\NR
    \NC\NC \cdots\NR
    \NC 2\cos(\alpha+ (n - 1)\beta)\sin\frac{\beta}{2} \NC = sin\left(\alpha + (2n - 1)\frac{\beta}{2}\right)
    - \sin\left(\alpha + (2n - 3)\frac{\beta}{2}\right)\NR
  \stopalign\stopformula

  Adding we get $2S\sin\frac{\beta}{2} = \sin\left(\alpha + (2n - 1)\frac{\beta}{2}\right) -
  \sin\left(\alpha - \frac{\beta}{2}\right)$

  $\Rightarrow S = \frac{\sin\frac{n\beta}{2}}{\sin\frac{\beta}{2}}\cos\left[\alpha + (n -
    1)\frac{\beta}{2}\right]$.
\item Let $S = \sin\theta + \sin3\theta + \sin5\theta + \cdots + \sin(2n - 1)\theta$

  Multiplying both sides by $2\sin\theta$ and writing in termwise fashion

  \startformula\startalign
    \NC 2\sin\theta\sin\theta \NC = 1 - \cos2\theta\NR
    \NC 2\sin\theta\sin3\theta \NC = \cos2\theta - \cos4\theta\NR
    \NC 2\sin\theta\sin5\theta \NC = \cos4\theta - \cos6\theta\NR
    \NC \NC \cdots\NR
    \NC 2\sin\theta\sin(2n - 1)\theta \NC = \cos(2n - 2)\theta - \cos2n\theta\NR
  \stopalign\stopformula

  Adding gives us $2S\sin\theta = 1 - \cos2n\theta = 2\sin^2n\theta$

  $\Rightarrow S = \frac{\sin^2n\theta}{\sin\theta}$.
\item The terms are of the form $\sin^2x$ which we can write as $\frac{1 - \cos2x}{2}$. Let the sum be $S$.

  Then $S = \frac{n}{2} - \frac{1}{2}\left[\cos2\alpha + \cos2(\alpha + \beta) + \cos2(\alpha + 2\beta) +
    \cdots + \cos2\left\{\alpha + (2n - 1)\beta\right\}\right]$

  Now we invoke the sum we obtained in second problem to arrive at

  $S = \frac{n}{2} - \frac{1}{2}\frac{\sin n\beta}{\sin\beta}\cos[2\alpha + (n - 1)\beta]$.
\item Since $B$ is the exterior angle of a regular polygon of $n$-sides. Thus, $B = \frac{2\pi}{n}$.

  L.H.S.\ $= \cos A + \cos\left(A + \frac{2\pi}{n}\right) + \cos\left(A + \frac{4\pi}{n}\right) + \cdots$ to
  $n$ terms

  $= \frac{\sin\pi}{\sin\frac{\pi}{n}}\cos\left[A + (n - 1)\frac{\pi}{n}\right]$.
\item $\because \sin(\pi + \theta) = -\sin\theta$ and $\sin(2\pi + \theta) = \sin\theta$

  $\Rightarrow -\sin(\alpha + \beta) = \sin(\pi + \alpha + \beta), \sin(\alpha + 2\beta) = \sin(2\pi +
  \alpha + 2\beta)$

  and $-\sin(\alpha + 3\beta) = \sin(3\pi + \alpha + 3\beta)$

  So we apply the formula obtained in first problem to get sum as $=
  \frac{\sin\frac{n\beta}{2}}{\sin\frac{\beta}{2}}\sin[\alpha + (n - 1)\beta]$.
\item Let $S = \sin\theta\sin2\theta + \sin2\theta\sin3\theta + \sin3\theta\sin4\theta + \cdots$

  $= \frac{1}{2}[(\cos\theta - \cos3\theta) + (\cos\theta - \cos5\theta) + (\cos\theta - \cos7\theta) +
  \cdots]$

  $= \frac{1}{2}[n\cos\theta - (\cos3\theta + \cos5\theta + \cos7\theta + \cdots)]$

  $= \frac{n}{2}\cos\theta - \frac{1}{2}\frac{\sin n\theta}{\sin\theta}\cos(n + 2)\theta$.
\item We have proven that $\cos\alpha + \cos(\alpha + \beta) + \cos(\alpha + 2\beta) + \cdots + \cos(\alpha
  + (n - 1)\beta) = \frac{\sin\frac{n\beta}{2}}{\sin\frac{\beta}{2}}\cos\left[\alpha + (n -
    1)\frac{\beta}{2}\right]$

  Comparing we have $\alpha = \frac{\pi}{11}, \beta = \frac{2\pi}{11}, n = 5$

  Thus, sum is $\frac{\sin\frac{5\pi}{11}}{\sin\frac{\pi}{11}}\cos\left[\frac{\pi}{11} +
    \frac{4\pi}{11}\right]$

  $= \frac{\sin\frac{5\pi}{11}}{\sin\frac{\pi}{11}}\cos\frac{5\pi}{11} =
  \frac{1}{2}\frac{\sin\frac{10\pi}{11}}{\sin\frac{\pi}{11}} = \frac{1}{2}\frac{\sin\left(\pi -
      \frac{\pi}{11}\right)}{\sin\frac{\pi}{11}} = \frac{1}{2}$.
\item Let $t_n$ denote the $n$th term. Then $t_1 = \frac{\sin x}{\sin2x\sin3x} = \frac{\sin(3x -
    2x)}{\sin2x\sin3x} = \cot2x - \cot3x$

  \startformula\startalign
    \NC t_1 \NC = \cot2x - \cot3x\NR
    \NC t_2 \NC = \cot3x - \cot4x\NR
    \NC t_3 \NC = \cot4x - \cot5x\NR
    \NC \NC \cdots\NR
    \NC t_n \NC = \cot(n + 1)x - \cot(n + 2)x\NR
  \stopalign\stopformula

  Adding and represeenting the sum as $S$, we have $S = \cot2x - \cot(n + 2)x$.
\item Let $t_n$ denote the $n$th term. Then $t_1 = \csc\theta\csc2\theta =
  \frac{1}{\sin\theta}.\frac{\sin\theta}{\sin\theta.\sin2\theta}$

  $= \frac{1}{\sin\theta}.\frac{\sin(2\theta - \theta)}{\sin\theta\sin2\theta} =
  \frac{1}{\sin\theta}[\cot\theta - \cot2\theta]$

  Now we proceed like previous problems to obtains the sum as $S = \frac{1}{\sin\theta}[\cot\theta - \cot(n
  + 1)\theta]$.
\item Let $t_n$ denote the $n$th term. Then $t_1 = \frac{1}{\cos\theta + \cos3\theta} =
  \frac{1}{2\cos2\theta\cos\theta}$

  $= \frac{1}{2}\frac{\sin\theta}{\cos2\theta\cos\theta\sin\theta} =
  \frac{1}{2\sin\theta}.\frac{\sin(2\theta - \theta)}{\cos2\theta\cos\theta} =
  \frac{1}{2\sin\theta}[\tan2\theta - \tan\theta]$

  \startformula\startalign
    \NC t_1\NC = \frac{1}{\sin\theta}[\tan2\theta - \tan\theta]\NR
    \NC t_2\NC = \frac{1}{\sin\theta}[\tan3\theta - \tan2\theta]\NR
    \NC t_3\NC = \frac{1}{\sin\theta}[\tan4\theta - \tan3\theta]\NR
    \NC \NC \cdots\NR
    \NC t_n\NC = \frac{1}{\sin\theta}[\tan(n + 1)\theta - \tan n\theta]\NR
  \stopalign\stopformula

  Adding and representing the sum as $S$, we have $S = \frac{1}{\sin\theta}[\tan(n + 1)\theta -
  \tan\theta]$.
\item Let $t_n$ denote the $n$th term. Then $t_1 = \frac{\sin x}{\cos x + \cos2x}$

  $= \frac{1}{2\sin\frac{x}{2}}.\frac{2\sin\frac{x}{2}\sin x}{\cos x + \cos 2x} =
  \frac{1}{2\sin\frac{x}{2}}.\frac{\cos\frac{x}{2} - \cos\frac{3x}{2}}{2\cos\frac{3x}{2}\cos\frac{x}{2}}$

  $= \frac{1}{4\sin\frac{x}{2}}\left[\sec\frac{3x}{2} - \sec\frac{x}{2}\right]$

  \startformula\startalign
    \NC t_1\NC = \frac{1}{4\sin\frac{x}{2}}\left[\sec\frac{3x}{2} - \sec\frac{x}{2}\right]\NR
    \NC t_2\NC = \frac{1}{4\sin\frac{x}{2}}\left[\sec\frac{5x}{2} - \sec\frac{3x}{2}\right]\NR
    \NC t_3\NC = \frac{1}{4\sin\frac{x}{2}}\left[\sec\frac{7x}{2} - \sec\frac{5x}{2}\right]\NR
    \NC \NC \cdots\NR
    \NC t_n\NC = \frac{1}{4\sin\frac{x}{2}}\left[\sec(2n + 1)\frac{x}{2} - \sec(2n - 1)\frac{x}{2}\right]\NR
  \stopalign\stopformula

  Adding and representing the sum as $S$, we have $S = \frac{\csc\frac{x}{2}}{4}\left[\sec(2n +
    1)\frac{x}{2} - \sec\frac{x}{2}\right]$.
\item We know that $\sin3\theta = 3\sin\theta - 4\sin^3\theta \Rightarrow 4\sin^3\theta = 3\sin\theta -
  \sin3\theta$

  \startformula\startalign
    \NC \sin^3\theta \NC = \frac{1}{4}[3\sin\theta - \sin3\theta]\NR
    \NC \frac{1}{3}\sin^33\theta \NC = \frac{1}{4}\left[\sin3\theta - \frac{1}{3}\sin9\theta\right]\NR
    \NC \frac{1}{3^2}\sin^39\theta \NC = \frac{1}{4}\left[\frac{1}{3}\sin9\theta - \frac{1}{3^2}\sin27\theta\right]\NR
    \NC \NC \cdots\NR
    \NC \frac{1}{3^{n - 1}}\sin\left(3^{n - 1}\theta\right) \NC = \frac{1}{4}\left[\frac{1}{3^{n -
          1}}\sin\left(3^{n - 1}\theta\right) - \frac{1}{3^{n - 1}}\sin3^n\theta\right]\NR
  \stopalign\stopformula

  Adding and representing the sum as $S$, we have $S = \frac{1}{4}\left[3\sin\theta - \frac{1}{3^{n -
        1}}\sin3^n\theta\right]$.
\item $\csc\theta = \frac{1}{\sin\theta} = \frac{1}{\sin\theta}.\frac{\sin\left(\theta -
  \frac{\theta}{2}\right)}{\sin\frac{\theta}{2}}$

  $= \frac{\sin\theta\cos\frac{\theta}{2} - \cos\theta\sin\frac{\theta}{2}}{\sin\theta\sin\frac{\theta}{2}}
  = \cot\frac{\theta}{2} - \cot\theta$

  \startformula\startalign
    \NC \csc\theta \NC = \cot\frac{\theta}{2} - \cot\theta\NR
    \NC \csc2\theta \NC = \cot\theta - \cot2\theta\NR
    \NC \csc2^2\theta \NC = \cot2\theta - \cot2^2\theta\NR
    \NC \NC \cdots\NR
    \NC \csc2^{n- 1}\theta \NC = \cot2^{n - 2}\theta - \cot2^{n - 1}\theta\NR
  \stopalign\stopformula

  Adding and representing the sum as $S$, we have $S = \cot\frac{\theta}{2} - \cot2^{n - 1}\theta$.
\item From previous problem we can say that

  \startformula\startalign
    \NC \csc\theta \NC = \cot\frac{\theta}{2} - \cot\theta\NR
    \NC \csc\frac{\theta}{2} \NC = \cot\frac{\theta}{2^2} - \cot\frac{\theta}{2}\NR
    \NC \csc\frac{\theta}{2^2} \NC = \cot\frac{\theta}{2^3} - \cot\frac{\theta}{2^2}\NR
    \NC \NC \cdots\NR
    \NC \csc\frac{\theta}{2^{n - 1}} \NC = \cot\frac{\theta}{2^n} - \cot\frac{\theta}{2^{n - 1}}\NR
  \stopalign\stopformula

  Adding and representing the sum as $S$, we have $S = \cot\frac{\theta}{2^n} - \cot\theta$.
\item $\tan(A - B) = \frac{\tan A - \tan B}{1 + \tan A\tan B}\Rightarrow \tan A\tan B = \cot(A - B)[\tan A -
  \tan B] - 1$. Thus, we can write

  \startformula\startalign
    \NC \tan x\tan2x\NC = \cot x[\tan2x - \tan x]- 1\NR
    \NC \tan2x\tan3x\NC = \cot x[\tan3x - \tan2x]- 1\NR
    \NC \tan3x\tan4x\NC = \cot x[\tan4x - \tan3x]- 1\NR
    \NC \NC \cdots\NR
    \NC \tan n\tan(n + 1)x\NC = \cot x[\tan(n + 1)x - \tan nx]- 1\NR
  \stopalign\stopformula

  Adding and representing the sum as $S$, we have $S = \cot x[\tan(n + 1)x - \tan nx] - n$.
\item $\tan x = \frac{\sin x}{\cos x} = \frac{\sin^2x}{\sin x\cos x} = \frac{\cos^2x - \left(\cos^2x -
  \sin^2x\right)}{\sin x\cos x}$

  $= \frac{\cos^2x}{\sin x\cos x} - \frac{2\cos2x}{\sin2x} = \cot x - 2\cot2x$

  Thus, we can write(we let $t_n$ represent the $n$th term)

  \startformula\startalign
    \NC t_1 \NC = \cot x - 2\cot2x\NR
    \NC t_2 \NC = 2\cot2x - 2^2\cot2^2x\NR
    \NC t_3 \NC = 2^2\cot2^2x - 2^3\cot2^3x\NR
    \NC \NC \cdots\NR
    \NC t_n \NC = 2^{n - 1}\cot2^{n - 1}x - 2^n\cot2^nx
  \stopalign\stopformula

  Adding and representing the sum as $S$, we have $S = \cot x - 2^n\cot2^nx$.
\item We can reuse the identity derives and write similarly

  \startformula\startalign
    \NC t_1 \NC = \cot\theta - 2\cot2\theta\NR
    \NC t_2 \NC = \frac{1}{2}\cot\frac{\theta}{2} - \cot\theta\NR
    \NC t_3 \NC = \frac{1}{2^2}\cot\frac{\theta}{262} - \frac{1}{2}\cot\frac{\theta}{2}\NR
    \NC \NC \cdots\NR
    \NC t_n \NC = \frac{1}{2^{n - 1}}\cot\frac{\theta}{2^{n - 1}} - \frac{1}{2^{n -
        2}}\cot\frac{\theta}{2^{n - 2}}\NR
  \stopalign\stopformula

  Adding and representing the sum as $S_n$, we have $S_n = \frac{1}{2^{n - 1}}\cot\frac{\theta}{2^{n - 1}} -
  2\cot2\theta$.

  $\displaystyle S_\infty = \lim_{n\to\infty}\left(\frac{1}{2^{n - 1}}\cot\frac{\theta}{2^{n - 1}} -
  2\cot2\theta\right)$

  $= \lim_{n\to\infty}\left[\frac{1}{\theta}.\frac{\theta}{2^{n - 1}}.\frac{1}{\tan\frac{\theta}{2^{n - 1}}}
    - 2\cot2\theta\right]$

  $= \frac{1}{\theta} - 2\cot2\theta$.
\item Let $S_n = \frac{1}{2}\sec x + \frac{1}{2^2}\sec x\sec2x + \frac{1}{2^3}\sec x\sec2x\sec2^2x +
  \cdots$ to $n$ terms

  $= \frac{1}{2\cos x} + \frac{1}{2^2\cos x\cos2x} + \frac{1}{2^3\cos x\cos2x\cos2^2x} + \cdots$ to $n$
  terms

  $= \frac{\sin x}{2\sin x\cos x} + \frac{\sin x}{2^2\sin x\cos x\cos2x} + \frac{\sin x}{2^3\sin x\cos
    x\cos2x\cos2^2x} + \cdots$ to $n$

  $= \sin x\left[\frac{1}{\sin 2x} + \frac{1}{\sin 4x} + \frac{1}{\sin 8x} + \cdots\right]$ to $n$ terms

  Now $\csc2x = \frac{1}{\sin2x} = \frac{\sin x}{\sin2x\sin x} = \frac{\sin(2x - x)}{\sin 2x\sin x} = \cot x
  - \cot 2x$

  Thus, we can write

  \startformula\startalign
    \NC \csc2x \NC = \cot x - \cot2x\NR
    \NC \csc4x \NC = \cot2x - \cot4x\NR
    \NC \csc8x \NC = \cot4x - \cot8x\NR
    \NC \NC \cdots\NR
    \NC csc2^nx \NC = \cot2^{n - 1}x - \cot2^nx\NR
  \stopalign\stopformula

  Adding we get $2S_n = \sin x[\cot x - \cot2^nx]$.
\item Let $t_n = \tan^{-1}\frac{nx}{1 + n(n + 1)x^2} = \tan^{-1}\frac{(n + 1)x - nx}{1 + [(n + 1)x]nx} =
  \tan^{-1}(n + 1)x - \tan^{-1}nx$

  Thus, we can write

  \startformula\startalign
    \NC t_1 \NC = \tan^{-1}2x - \tan^{-1}x\NR
    \NC t_2 \NC = \tan^{-1}3x - \tan^{-1}2x\NR
    \NC t_3 \NC = \tan^{-1}4x - \tan^{-1}3x\NR
    \NC \NC \cdots\NR
    \NC t_n \NC = \tan^{-1}(n + 1)x - \tan^{-1}nx\NR
  \stopalign\stopformula

  Adding and representing the sum as $S$, we have $S = \tan^{-1}(n + 1)x - \tan^{-1}x$.
\item Let $t_n$ denote the $n$th term of the series. Then $t_n = \tan^{-1}\frac{1}{2n^2} =
  \tan^{-1}\frac{2}{4n^2}$

  $= \tan^{-1}\left[\frac{(2n + 1) - (2n - 1)}{1 + (2n + 1)(2n - 1)}\right] = \tan^{-1}(2n + 1) -
  \tan^{-1}(2n - 1)$

  Thus, we can write

  \startformula\startalign
    \NC t_1 \NC = \tan^{-1}3 - \tan^{-1}1\NR
    \NC t_2 \NC = \tan^{-1}5 - \tan^{-1}3\NR
    \NC t_3 \NC = \tan^{-1}7 - \tan^{-1}5\NR
    \NC \NC \cdots\NR
    \NC t_n \NC = \tan^{-1}(2n + 1) - \tan^{-1}(2n - 1)\NR
  \stopalign\stopformula

  Adding and representing the sum as $S_n$, we have $S_n = \tan^{-1}(2n + 1) - \tan^{-1}1$

  Now $\displaystyle S_\infty = \lim_{n\to\infty}\left(\tan^{-1}(2n + 1) - \tan^{-1}1\right) = \frac{\pi}{2}
  - \frac{\pi}{4} = \frac{\pi}{4}$.
\item Let $t_n$ denote the $n$th term. $t_n = \tan^{-1}\frac{1}{3 + 3n + n^2} = \tan^{-1}\frac{1}{1 + n^2 +
  3n + 2}$

  $=\tan^{-1}\frac{1}{1 + (n + 2)(n + 1)} = \tan^{-1}(n + 2) - \tan^{-1}(n + 1)$

  Thus, we can write

  \startformula\startalign
    \NC t_1 \NC = \tan^{-1}3 - \tan^{-1}2\NR
    \NC t_2 \NC = \tan^{-1}4 - \tan^{-1}3\NR
    \NC t_3 \NC = \tan^{-1}5 - \tan^{-1}4\NR
    \NC \NC \cdots\NR
    \NC t_n \NC = \tan^{-1}(n + 2) - \tan^{-1}(n + 1)\NR
  \stopalign\stopformula

  Adding and representing the sum as $S$, we have $S = \tan^{-1}(n + 2) - \tan^{-1}2$.
\item Let $t_n$ represent the $n$th term. Then $t_n = \sin^{-1}\left[\frac{\sqrt{n} - \sqrt{n -
      1}}{\sqrt{n}\sqrt{n + 1}}\right]$

  $= \sin^{-1}\left[\frac{\sqrt{n}}{\sqrt{n}\sqrt{n + 1}} - \frac{\sqrt{n - 1}}{\sqrt{n}\sqrt{n + 1}}\right]
  = \sin^{-1}\left[\frac{1}{\sqrt{n}}\sqrt{1 - \frac{1}{n + 1}} - \frac{1}{\sqrt{n + 1}}\sqrt{1 -
      \frac{1}{n}}\right]$

  Let $\frac{1}{\sqrt{n}} = \sin A$ and $\frac{1}{\sqrt{n + 1}} = \sin B$ then $\cos A = \sqrt{1 -
    \frac{1}{n}}$ and $\cos B = \sqrt{1 - \frac{1}{n + 1}}$

  $\Rightarrow t_n = \sin^{-1}[\sin A\cos B - \sin B\cos A] = \sin^{-1}\sin(A - B) = A - B =
  \sin^{-1}\frac{1}{\sqrt{n}} - \sin^{-1}\frac{1}{\sqrt{n + 1}}$

  Thus, we can write

  \startformula\startalign
    \NC t_1 \NC = \sin^{-1}1 - \sin^{-1}\frac{1}{\sqrt{2}}\NR
    \NC t_2 \NC = \sin^{-1}\frac{1}{\sqrt{2}} - \sin^{-1}\frac{1}{\sqrt{3}}\NR
    \NC t_3 \NC = \sin^{-1}\frac{1}{\sqrt{3}} - \sin^{-1}\frac{1}{\sqrt{4}}\NR
    \NC \NC \cdots\NR
    \NC t_n \NC = \sin^{-1}\frac{1}{\sqrt{n}} - \sin^{-1}\frac{1}{\sqrt{n + 1}}\NR
  \stopalign\stopformula

  Adding and representing the sum as $S$, we have $S = \sin^{-1}1 - \sin^{-1}\frac{1}{\sqrt{n + 1}}$

  $\displaystyle\lim_{n\to\infty}S = \frac{\pi}{2}$.
\item Let $C = \cos\alpha + x\cos(\alpha + \beta) + \frac{x^2}{2!}\cos(\alpha + 2\beta) +
  \cdots$ to $\infty$

  and $S = \sin\alpha + x\sin(\alpha + \beta) + \frac{x^2}{2!}\sin(\alpha + 2\beta) +
  \cdots$ to $\infty$

  $C + iS = e^{i\alpha} + xe^{i(\alpha + \beta)} + \frac{x^2}{2!}e^{i(\alpha + 2\beta)} + \cdots$ to
  $\infty$

  $= e^{i\alpha}\left[1 + xe^{i\beta} + \frac{x^2}{2!}e^{i2\beta} + \cdots \text{ to } \infty\right]$

  $= e{i\alpha}\left[1 + z + \frac{z^2}{2!} + \cdots \text{ to } \infty\right]$ where $z = x.e^{i\beta}$

  $= e^{i\alpha}e^{xe^{i\beta}} = e^{i\alpha}e^{x\cos\beta}e^{i\sin\beta} = e^{x\cos\beta}[\cos(\alpha +
    x\sin\beta) + i\sin(\alpha + i\sin\beta)]$

  Comparing real parts we have $C = e^{x\cos\beta}\cos(\alpha + x\sin\beta)$.
\item Let $C = \cos\theta - \frac{\cos2\theta}{2!} + \frac{\cos3\theta}{3!} - \cdots$ to $\infty$

  and $S = \sin\theta - \frac{\sin2\theta}{2!} + \frac{\sin3\theta}{3!} - \cdots$ to
  $\infty$

  Then $C + iS = (\cos\theta + i\sin\theta) - \frac{\cos2\theta + i\sin2\theta}{2!} + \frac{\cos3\theta +
    i\sin3\theta}{3!} - \cdots$ to $\infty$

  $= e^{i\theta} - \frac{e^{i2\theta}}{2!} + \frac{e^{i3\theta}}{3!} + \cdots$ to $\infty = 1 -
  e^{-i\theta}$

  $= 1 - e^{-(\cos\theta + i\sin\theta)} = 1 - e^{-\cos\theta}e^{-i\sin\theta} = 1 -
  e^{-\cos\theta}[\cos(\sin\theta) - i\sin(\sin\theta)]$

  Comparing imaginary parts $C = e^{-\cos\theta}\sin(\sin\theta)$.
\item Let $S = \sin\theta\cos\theta + \frac{\sin2\theta\cos^2\theta}{2!} +
  \frac{\sin3\theta\cos^3\theta}{3!} + \cdots $ to $\infty$

  and $C = 1 + \cos\theta\cos\theta + \frac{\cos2\theta\cos^2\theta}{2!} +
  \frac{\cos3\theta\cos^2\theta}{3!} + \cdots$ to $\infty$

  Now $C + iS = 1 + \cos\theta e^{i\theta} + \frac{\cos^2\theta}{2!}e^{i2\theta} +
  \frac{\cos^3\theta}{3!}e^{i3\theta} + \cdots$ to $\infty$

  $= 1 + z + \frac{z^2}{2!} + \frac{z^3}{3!} + \cdots$ to $\infty$[where $z = \cos\theta e^{i\theta}$]

  $ = e^z = e^{\cos\theta e^{i\theta}} = e^{\cos^2\theta}e^{i\sin\theta\cos\theta} =
  e^{\cos^2\theta}[\cos(\sin\theta\cos\theta) + i\sin(\sin\theta\cos\theta)]$

  Comparing imaginary parts $S = e^{\cos^2\theta}\sin(\sin\theta\cos\theta)$.
\item Let $C = \cos\theta + \frac{\sin\theta}{1!}\cos2\theta + \frac{\sin^2\theta}{2!}\cos3\theta +
  \frac{\sin^3\theta}{3!}\cos4\theta + \cdots$ to $\infty$

  and $S = \sin\theta + \frac{\sin\theta}{1!}\sin2\theta + \frac{\sin^2\theta}{2!}\sin3\theta +
  \frac{\sin^3\theta}{3!}\sin4\theta + \cdots$ to $\infty$

  $C + iS = e^{i\theta} + \frac{\sin\theta}{1!}e^{i2\theta} + \frac{\sin^2\theta}{2!}e^{i3\theta} + \cdots$
  to $\infty$

  $= e^{i\theta}\left[1 + \frac{\sin\theta}{1!}e^{i\theta} + \frac{\sin^2\theta}{2!}e^{i2\theta} + \cdots
    \infty\right]$

  $= e^{i\theta}\left[1 + z + \frac{z^2}{2!} + \frac{z^3}{3!} + \cdots \infty\right]$ where $z = \sin\theta
  e^{i\theta}$

  $= e^{i\theta}e^z = e^{i\theta}e^{\sin\theta e^{i\theta}} = e^{i\theta}e^{\sin\theta(\cos\theta +
    i\sin\theta)}$

  $= e^{\sin\theta\cos\theta}e^{i(\theta + \sin^2\theta)} = e^{\sin\theta\cos\theta}[cos(\theta +
    \sin^2\theta) + i\sin(\theta + \cos^2\theta)]$

  Comparing real parts, we have sum as $C = e^{\sin\theta\cos\theta}\cos(\theta + \sin^2\theta)$.
\item Let $C = x\cos\theta + \frac{x^2}{2}\cos2\theta + \frac{x^3}{\theta}\cos3\theta +
  \cdots$ to $\infty$

  and $S = x\sin\theta + \frac{x^2}{2}\sin2\theta + \frac{x^3}{\theta}\sin3\theta +
  \cdots$ to $\infty$

  $C + iS = xe^{i\theta} + \frac{x^2}{2}e^{i2\theta} + \frac{x^3}{3}e^{i3\theta} + \cdots$ to $\infty$

  $= z + \frac{z^2}{2} + \frac{z^3}{3} + \cdots$ to $\infty$ where $z = xe^{i\theta}$

  $= -\log_e(1 - z) = -\log_e\left(1 - xe^{i\theta}\right) = -\log_e[(1 - x\cos\theta) - ix\sin\theta]$

  We know that $\log_e(\alpha + \beta) = \frac{1}{2}\log_e\left(\alpha^2 + \beta^2\right) +
  i\tan^{-1}\frac{\beta}{\alpha}$

  Using the formula above we can write

  $C + iS = -\left[\frac{1}{2}\log_e\left\{(1 - x\cos\theta)^2 + x^2\sin^2\theta\right\} -
    i\tan^{-1}\frac{x\sin\theta}{1 - x\cos\theta}\right]$

  Comparing real parts we get $C = -\frac{1}{2}\log_e(1 - 2x\cos\theta + x^2)$.
\item We proceed like previous problem and compare imaginary parts to obtain the sum as $S =
  \tan^{-1}\frac{x\sin\theta}{1 - x\cos\theta}$.
\item Let $C = \cos\theta + \frac{\cos2\theta}{2} + \frac{\cos3\theta}{3} +
  \frac{\cos4\theta}{4} + \cdots$ to $\infty$

  and $S = \sin\theta - \frac{1}{2}\sin2\theta + \frac{1}{3}\sin3\theta - \cdots \infty$

  $\Rightarrow C + iS = e^{i\theta} - \frac{1}{2}e^{i2\theta} + \frac{1}{3}e^{i3\theta} - \cdots \infty$

  $= \log_e\left(1 + e^{i\theta}\right) = \log_e(1 + \cos\theta + i\sin\theta)$

  $= \frac{1}{2}\log_e\left[(1 + \cos\theta)^2 + \sin^2\theta\right] + i\tan^{-1}\frac{\sin\theta}{1 +
    \cos\theta}$

  $ = \frac{1}{2}\log_e\left(4\cos^2\frac{\theta}{2}\right) + i\tan^{-1}\tan\frac{\theta}{2} =
  \log_e\left(2\cos\frac{\theta}{2}\right) + i\frac{\theta}{2}$

  Comparing real parts, we get $C = \log_e\left(2\cos\frac{\theta}{2}\right)$.
\item Let $C = \cos\frac{\pi}{3} + \frac{1}{2}\cos\frac{2\pi}{3} + \frac{1}{3}\cos\frac{3\pi}{3} +
  \cdots$ to $\infty = 0$

  and $S = \sin\frac{\pi}{3} + \frac{1}{2}\sin\frac{2\pi}{3} + \frac{1}{3}\sin\frac{3\pi}{3} + \cdots$ to
  $\infty$

  $\Rightarrow C + iS = e^{i\frac{\pi}{3}} + \frac{1}{2}e^{i\frac{2\pi}{3}} + \frac{1}{3}e^{i\frac{3\pi}{3}}
  + \cdots$ to $\infty$

  $= -\log_e\left(1 - e^{i\frac{\pi}{3}}\right) = -\log_e\left[1 - \left(\cos\frac{\pi}{3} +
    i\sin\frac{\pi}{3}\right)\right] = -\log_e\left[\frac{1}{2} - i\frac{\sqrt{3}}{2}\right]$

  $= -\frac{1}{2}\log_e\left(\frac{1}{3} + \frac{3}{4}\right) -i\tan^{-1}\sqrt{3} = 0 + i\frac{\pi}{3}$

  Comparing real and imaginary parts $C = 0, S = \frac{\pi}{3}$.
\item Let $S = \sin\alpha + n\sin(\alpha + \beta) + \frac{n(n - 1)}{2!}\sin(\alpha + 2\beta) + \cdots$ upto
  $(n + 1)$ terms

  and $C = \cos\alpha + n\cos(\alpha + \beta) + \frac{n(n - 1)}{2!}\cos(\alpha + 2\beta) + \cdots$ upto $(n
  + 1)$ terms

  $C + iS = e^{i\alpha} + ne^{i(\alpha + \beta)} + \frac{n(n - 1)}{2}e^{i(\alpha + 2\beta)} + \cdots$

  $= e^{i\alpha}\left[1 + ne^{i\beta} + \frac{n(n - 1)}{2}e^{i2\beta} + \cdots\right] = e^{i\alpha}\left(1 +
  e^{ii\beta}\right)^n$

  $= e^{i\alpha}\left[\left(1 + \cos\beta + i\sin\beta\right)^n\right] =
  e^{i\alpha}\left[2\cos^2\frac{\beta}{2} + i.2\sin\frac{\beta}{2}\cos\frac{\beta}{2}\right]^n$

  $= e^{i\alpha}\left(2\cos\frac{\beta}{2}\right)^ne^{in\frac{\beta}{2}} =
  2^n\cos^n\frac{\beta}{2}\left[\cos\left(\alpha + \frac{n\beta}{2}\right) + i\sin\left(\alpha +
    \frac{n\beta}{2}\right)\right]$

  Equating imaginary paarts gives us

  $S = 2^n\cos^n\frac{\beta}{2}\sin\left(\alpha + \frac{n\beta}{2}\right)$.
\stopitemize